

# CSE 400 — Lecture 11 Scribe

Fundamentals of Probability in Computing  
Lecture 11: Transformation of Random Variables

## 1 Transformation of Random Variables

### 1.1 Problem Setting

Let  $X$  be a continuous random variable (CRV) with known:

PDF:  $f_X(x)$

CDF:  $F_X(x)$

These are assumed known a priori.

Define a new random variable:

$$Y = g(X)$$

The objective is to determine:

$$F_Y(y), \quad f_Y(y)$$

The transformation is treated under the assumption of monotonicity of  $g(\cdot)$ .

Two cases arise:

- Monotonically increasing
- Monotonically decreasing

### 1.2 Step 1: CDF Method

$$F_Y(y) = P(Y \leq y)$$

Since  $Y = g(X)$ ,

$$F_Y(y) = P(g(X) \leq y)$$

The next step depends on monotonicity of  $g(\cdot)$ .

#### Case 1: Monotonically Increasing

If  $g$  is increasing:

$$g(X) \leq y \iff X \leq g^{-1}(y)$$

Thus,

$$F_Y(y) = P(X \leq g^{-1}(y)) = F_X(g^{-1}(y))$$

Differentiate to obtain PDF:

$$f_Y(y) = \frac{d}{dy} F_Y(y) = \frac{d}{dy} F_X(g^{-1}(y))$$

Using chain rule:

$$f_Y(y) = f_X(g^{-1}(y)) \cdot \frac{d}{dy} g^{-1}(y)$$

Equivalently written:

$$f_Y(y) = f_X(x) \frac{dx}{dy} \quad \text{evaluated at } x = g^{-1}(y)$$

### Case 2: Monotonically Decreasing

If  $g$  is decreasing:

$$g(X) \leq y \iff X \geq g^{-1}(y)$$

Thus,

$$F_Y(y) = P(X \geq g^{-1}(y)) = 1 - F_X(g^{-1}(y))$$

Differentiate:

$$\begin{aligned} f_Y(y) &= \frac{d}{dy} [1 - F_X(g^{-1}(y))] \\ &= -f_X(g^{-1}(y)) \cdot \frac{d}{dy} g^{-1}(y) \end{aligned}$$

Since  $\frac{d}{dy} g^{-1}(y) < 0$ ,

$$f_Y(y) = f_X(x) \frac{dx}{dy} \quad \text{evaluated at } x = g^{-1}(y)$$

## 1.3 Change of Limits

Adjust limits according to the mapping  $y = g(x)$ .

The support of  $Y$  is determined by transforming the support of  $X$ .

## 2 Worked Example

Given:

$$X \sim \text{Uniform}(-1, 1)$$

$$f_X(x) = \begin{cases} \frac{1}{2}, & -1 < x < 1 \\ 0, & \text{otherwise} \end{cases}$$

Define:

$$Y = \sin\left(\frac{\pi X}{2}\right)$$

Find  $f_Y(y)$ .

### Step 1: Inverse Transformation

$$X = \frac{2}{\pi} \sin^{-1}(Y)$$

### Step 2: Derivative

$$\frac{dx}{dy} = \frac{2}{\pi} \cdot \frac{1}{\sqrt{1-y^2}}$$

### Step 3: Apply Transformation Formula

$$f_Y(y) = f_X(x) \frac{dx}{dy}$$

Substitute  $f_X(x) = \frac{1}{2}$ :

$$f_Y(y) = \frac{1}{2} \cdot \frac{2}{\pi} \cdot \frac{1}{\sqrt{1-y^2}}$$

$$f_Y(y) = \frac{1}{\pi \sqrt{1-y^2}}$$

Support:

Since  $x \in (-1, 1)$ ,

$$y \in (-1, 1)$$

Final answer:

$$f_Y(y) = \begin{cases} \frac{1}{\pi \sqrt{1-y^2}}, & -1 < y < 1 \\ 0, & \text{otherwise} \end{cases}$$

## 3 Function of Two Random Variables

Let:

$$Z = X + Y$$

Goal:

1. Find  $f_Z(z)$ .
2. If  $X$  and  $Y$  are independent, find  $f_Z(z)$ .
3. If  $X, Y \sim N(0, 1)$ , prove  $Z \sim N(0, 2)$ .
4. If exponential with parameter  $\lambda$ , find  $f_Z(z)$ .

## 4 Derivation of $f_Z(z)$

### Step 1: CDF Method

$$F_Z(z) = P(Z \leq z) = P(X + Y \leq z)$$

Region:

$$\{(x, y) : x + y \leq z\}$$

Line:

$$x + y = z$$

Region below the line.

### Step 2: Double Integral Form

$$F_Z(z) = \int_{-\infty}^{\infty} \int_{-\infty}^{z-y} f_{XY}(x, y) dx dy$$

Equivalently (order switched):

$$F_Z(z) = \int_{-\infty}^{\infty} \int_{-\infty}^{z-x} f_{XY}(x, y) dy dx$$

### Step 3: If $X$ and $Y$ Independent

$$f_{XY}(x, y) = f_X(x)f_Y(y)$$

Thus,

$$f_Z(z) = \int_{-\infty}^{\infty} f_X(x)f_Y(z-x) dx$$

This is the convolution form for the PDF of  $Z = X + Y$ .

## 5 Summary of Core Results

### Single Variable Transformation

If  $Y = g(X)$  and  $g$  is monotone:

$$f_Y(y) = f_X(g^{-1}(y)) \frac{d}{dy} g^{-1}(y)$$

### Sum of Two Random Variables

$$F_Z(z) = P(X + Y \leq z)$$

If independent:

$$f_Z(z) = \int_{-\infty}^{\infty} f_X(x)f_Y(z-x) dx$$